books/kestrel/axe/risc-v/lifter-rules.lisp
@@ -1,0 +1,149 @@
+; Rules for lifting
+;
+; Copyright (C) 2016-2019 Kestrel Technology, LLC
+; Copyright (C) 2025 Kestrel Institute
+;
+; License: A 3-clause BSD license. See the file books/3BSD-mod.txt.
+;
+; Author: Eric Smith (eric.smith@kestrel.edu)
+
+;;;;;;;;;;;;;;;;;;;;;;;;;;;;;;;;;;;;;;;;;;;;;;;;;;;;;;;;;;;;;;;;;;;;;;;;;;;;;;;;
+
+(in-package "R")
+
+(include-book "read-and-write")
+(include-book "kestrel/axe/known-booleans" :dir :system)
+(include-book "../priorities")
+(local (include-book "kestrel/bv/unsigned-byte-p" :dir :system))
+
+(add-known-boolean in-region32p)
+(add-known-boolean subregion32p)
+(add-known-boolean disjoint-regions32p)
+
+(add-known-boolean stat32ip)
+
+(def-constant-opener in-region32p)
+(def-constant-opener subregion32p)
+(def-constant-opener disjoint-regions32p)
+
+;;;;;;;;;;;;;;;;;;;;;;;;;;;;;;;;;;;;;;;;;;;;;;;;;;;;;;;;;;;;;;;;;;;;;;;;;;;;;;;;
+
+(def-constant-opener riscv::decodex)
+(def-constant-opener ubyte32-fix)
+(def-constant-opener ubyte32p)
+(def-constant-opener riscv::get-fields-itype)
+(def-constant-opener riscv::get-fields-jtype)
+(def-constant-opener riscv::get-rd)
+(def-constant-opener riscv::get-rs1)
+(def-constant-opener riscv::get-rs2)
+(def-constant-opener riscv::get-funct3)
+(def-constant-opener riscv::get-funct7)
+
+(def-constant-opener riscv::get-opcode)
+(def-constant-opener riscv::get-imm-btype)
+(def-constant-opener riscv::get-imm-itype)
+(def-constant-opener riscv::get-imm-jtype)
+(def-constant-opener riscv::get-imm-stype)
+(def-constant-opener riscv::get-imm-utype)
+(def-constant-opener bitops::part-select-low-high$inline)
+(def-constant-opener bitops::part-select-width-low$inline)
+(def-constant-opener riscv::feat-64p)
+(def-constant-opener riscv::get-fields-rtype)
+(def-constant-opener riscv::get-fields-btype)
+(def-constant-opener riscv::get-fields-utype)
+(def-constant-opener riscv::get-fields-stype)
+(def-constant-opener riscv::feat->m$inline)
+
+(def-constant-opener logtail$inline)
+(def-constant-opener expt2$inline)
+(def-constant-opener ifloor$inline)
+(def-constant-opener logapp)
+(def-constant-opener binary-logand)
+(def-constant-opener ash)
+
+(def-constant-opener riscv::instr-op-imm)
+(def-constant-opener riscv::op-imm-funct-kind$inline)
+
+(def-constant-opener riscv::instr-store)
+(def-constant-opener riscv::instr-load)
+(def-constant-opener riscv::instr-op)
+
+
+;todo: more
+(defopeners exec32-op-imm :hyps ((syntaxp (quotep riscv::funct))))
+
+
+;;;;;;;;;;;;;;;;;;;;;;;;;;;;;;;;;;;;;;;;;;;;;;;;;;;;;;;;;;;;;;;;;;;;;;;;;;;;;;;;
+
+;move and gen
+
+;; may help with sbox lookup, etc.
+(defthm in-region32p-byte-special
+  (implies (and (unsigned-byte-p 8 x)
+                (<= 256 len)
+                (natp len))
+           (in-region32p x len 0))
+  :hints (("Goal" :in-theory (enable in-region32p bvlt))))
+
+(defthm disjoint-regions32p-byte-special
+  (implies (and (syntaxp (and (quotep ad)
+                              (quotep len)))
+                (unsigned-byte-p 32 len)
+                (unsigned-byte-p 32 ad)
+                (bvlt 32 255 ad)
+                (bvle 32 len (bvminus 32 (+ -1 (expt 2 32)) ad))
+                (integerp ad)
+                (natp len)
+                (unsigned-byte-p 8 byte))
+           (disjoint-regions32p 1 byte len ad))
+  :hints (("Goal" :in-theory (enable disjoint-regions32p bvlt bvminus unsigned-byte-p acl2::bvchop-of-sum-cases))))
+
+;move acl2::bvminus-becomes-bvplus-of-bvuminus-constant-version out of axe/rules3.
+
+;;special case for isize=8
+(defthmd bv-array-read-shorten-8
+  (implies (and (unsigned-byte-p 8 index)
+                (< (expt 2 8) len)
+                (equal len (len data)))
+           (equal (bv-array-read element-size len index data)
+                  (bv-array-read element-size (expt 2 8) index (take (expt 2 8) data))))
+  :hints (("Goal" :use (:instance acl2::bv-array-read-shorten-core (isize 8) (index index) (data data) (element-size element-size))
+           :in-theory (disable acl2::bv-array-read-shorten-core))))
+
+;; todo: arrange to (safely) eval binary-logand
+
+(defthm not-in-region32p-when-disjoint-regions32p-special
+  (implies (and (disjoint-regions32p len1 ad1 len2 ad) ; ad here is the same as in the lhs
+                (posp len2)
+                (subregion32p len start len1 ad1))
+           (not (in-region32p ad len start))))
+
+
+(defun bvlt-alias (size x y) (bvlt size x y))
+
+(defthm show-unresolved-bvlt
+  (implies (bvlt-alias size x y)
+           (bvlt size x y)))
+;; try very late
+(acl2::set-axe-rule-priority show-unresolved-bvlt 10)
+
+
+;;(thm (not (bvlt '32 (bvplus '32 '4294960416 (bvxor '8 x y)) '4)))
+
+(defthm <-of-read-linear
+  (implies (natp n)
+           (< (read n addr stat) (expt 2 (* 8 n))))
+  :rule-classes :linear
+  :hints (("Goal" :use (unsigned-byte-p-of-read-simple)
+           :in-theory (disable unsigned-byte-p-of-read
+                               unsigned-byte-p-of-read-simple))))
+
+(defthm bvlt-of-read-and-constant
+  (implies (and (syntaxp (and (quotep k)
+                              (quotep size)
+                              (quotep n)))
+                (<= (expt 2 (* 8 n)) (bvchop size k))
+                (natp n)
+                (natp size))
+           (bvlt size (read n addr stat) k))
+  :hints (("Goal" :in-theory (enable bvlt))))
